theories/rules/donate.v
@@ -249,14 +249,14 @@ Lemma hvc_donate_z {instr i wi r2 pi ptx sown q sacc sexcl des sh wss} {l :Word}
   {SS{{ ▷(PC @@ i ->r ai) ∗ ▷ ai ->a wi
   ∗ ▷ O@i:={q}[sown] ∗ ▷ A@i:={1}[sacc] ∗ ▷ E@i:={1}[sexcl]
   ∗ ▷ (R0 @@ i ->r r0) ∗ ▷ (R1 @@ i ->r r1) ∗ ▷(R2 @@i ->r r2) ∗  ▷ TX@ i := ptx
-  ∗ ▷ mem_region des ptx ∗ ▷ ([∗ list] p;ws ∈ psd;wss, mem_region ws (of_pid p))
+  ∗ ▷ mem_region des ptx ∗ ▷ ([∗ list] p;ws ∈ psd;wss, mem_page ws p)
   ∗ ▷ hp{ 1 }[ sh ] }}}
    ExecI @ i {{{ RET ExecI ; PC @@ i ->r (ai ^+ 1)%f ∗ ai ->a wi
   ∗ O@i:={q}[sown] ∗ A@i:={1}[sacc∖spsd] ∗ E@i:={1}[sexcl∖spsd]
   ∗ R0 @@ i ->r (encode_hvc_ret_code Succ) ∗ R1 @@ i ->r r1  ∗ TX@ i := ptx
   ∗ ∃(wh: Word), ( ⌜ wh ∈ sh ⌝ ∗ R2 @@ i ->r wh ∗ wh ->t{1}(i,W1, j , psd,Donation)
   ∗ wh ->re false  ∗ hp{1}[ (sh∖{[wh]})] )
-  ∗ mem_region des ptx ∗ ([∗ list] p ∈ psd, mem_region list_of_W0 (of_pid p) )}}}.
+  ∗ mem_region des ptx ∗ ([∗ list] p;ws ∈ psd;(pages_of_W0 (length psd)), mem_page ws p)}}}.
 Proof.
   iIntros (Hinstr Hdecodei Hini Hdecodef Hneq Hlenpsd Hdesc Hindesc Hlenr1 Hspsd Hsacc Hsown Hsexcl Hshne Φ ).
   iIntros "(>PC & >Hai & >Hown & >Hacc & >Hexcl & >R0 & >R1 & >R2 & >TX & >Hadesc & >Hpgs & >Hhp ) HΦ".
@@ -359,8 +359,6 @@ Proof.
         solve_reg_lookup.
         done.
      }
-     (* 2 : { rewrite ?update_reg_global_preserve_current_vm  ?update_access_batch_preserve_current_vm *)
-     (*        ?zero_pages_preserve_current_vm ?insert_transaction_preserve_current_vm //. } *)
      2 : {
         rewrite !update_reg_global_update_reg.
         rewrite ?update_access_batch_preserve_regs
@@ -383,8 +381,9 @@ Proof.
      iDestruct ((gen_reg_update3_global PC i (ai ^+ 1)%f R2 i h R0 i (encode_hvc_ret_code Succ) ) with "Hσreg PC R2 R0") as ">[Hσreg [PC [R2 R0]]]";eauto.
      rewrite Hcureq.
      iFrame.
-     (* TODO: update memory *)
-     iDestruct ((gen_mem_update_pages σ1 psd list_of_W0) with "Hσmem Hpgs") as ">[Hσmem Hpgs]";eauto.
+     iDestruct ((gen_mem_update_pages σ1 psd (pages_of_W0 (length psd))) with "Hσmem Hpgs") as ">[Hσmem Hpgs]";eauto.
+     { apply length_pages_of_W0_forall. }
+     { rewrite length_pages_of_W0 //. }
      (* update page table *)
      rewrite (@update_access_batch_update_access_diff _ i sacc spsd psd);eauto.
      rewrite ?zero_pages_preserve_current_vm ?insert_transaction_preserve_current_vm.
@@ -442,8 +441,5 @@ Proof.
      iFrame.
      done.
 Qed.
-
-
-
 
 End donate.
